HS_Lie_Derivatives.thy
@@ -328,8 +328,8 @@ thm expr_differentiable_when_on_def
 lemma lie_diff_inv_on_eq:
   fixes e :: "'s \<Rightarrow> _::real_inner" and a :: "'c::real_normed_vector \<Longrightarrow> 's"
   assumes "vwb_lens a" "differentiable\<^sub>e e on a" "`B \<longrightarrow> \<L>\<^bsub>F\<^esub> e on a = 0`"
-  shows "diff_inv_on (e = 0)\<^sub>e a (\<lambda> _. F) ({t. t \<ge> 0})\<^sub>e UNIV 0 (B)\<^sub>e"
-  using assms apply(simp_all add: diff_inv_on_eq ivp_sols_def)
+  shows "diff_inv_on a (\<lambda> _. F) (B)\<^sub>e ({t. t \<ge> 0})\<^sub>e UNIV 0 (e = 0)\<^sub>e"
+  using assms apply(simp_all add: diff_inv_on_eq ivp_sols_def tsubst2vecf_eq)
 proof(auto simp: lens_defs expr_defs)
   fix t :: real and X :: "real \<Rightarrow> 'c" and s :: "'s"
   assume a1:"\<forall>s. (\<lambda>x. e (put\<^bsub>a\<^esub> s x)) differentiable at (get\<^bsub>a\<^esub> s)" and a2: "0 \<le> t" 
@@ -382,9 +382,9 @@ lemma lie_diff_inv_simple:
 lemma lie_diff_inv_on_le_less:
   fixes e :: "'s \<Rightarrow> real" and a :: "'c::real_normed_vector \<Longrightarrow> 's"
   assumes "vwb_lens a" "differentiable\<^sub>e e on a" "`B \<longrightarrow> \<L>\<^bsub>F\<^esub> e on a \<ge> 0`"
-  shows lie_diff_inv_on_leq: "diff_inv_on (e \<ge> 0)\<^sub>e a (\<lambda> _. F) ({t. t \<ge> 0})\<^sub>e UNIV 0 (B)\<^sub>e"
-    and lie_diff_inv_on_less: "diff_inv_on (e > 0)\<^sub>e a (\<lambda> _. F) ({t. t \<ge> 0})\<^sub>e UNIV 0 (B)\<^sub>e"
-  using assms apply(simp_all add: diff_inv_on_eq ivp_sols_def)
+  shows lie_diff_inv_on_leq: "diff_inv_on a (\<lambda> _. F) (B)\<^sub>e ({t. t \<ge> 0})\<^sub>e UNIV 0 (e \<ge> 0)\<^sub>e"
+    and lie_diff_inv_on_less: "diff_inv_on a (\<lambda> _. F) (B)\<^sub>e ({t. t \<ge> 0})\<^sub>e UNIV 0 (e > 0)\<^sub>e"
+  using assms apply(simp_all add: diff_inv_on_eq ivp_sols_def tsubst2vecf_eq)
 proof(auto simp: lens_defs expr_defs)
   fix t :: real and X :: "real \<Rightarrow> 'c" and s :: "'s"
   assume a1:"\<forall>s. (\<lambda>x. e (put\<^bsub>a\<^esub> s x)) differentiable at (get\<^bsub>a\<^esub> s)" and a2: "0 \<le> t" 
@@ -421,9 +421,10 @@ qed
 lemma lie_deriv_eq_rule:
   fixes e :: "'s \<Rightarrow> 'a::real_inner" and a :: "'c::real_normed_vector \<Longrightarrow> 's"
   assumes "vwb_lens a" "differentiable\<^sub>e e on a" "differentiable\<^sub>e f on a"
-  shows lie_deriv_eq: "`B \<longrightarrow> \<L>\<^bsub>F\<^esub> e on a = \<L>\<^bsub>F\<^esub> f on a` \<Longrightarrow> diff_inv_on (e = f)\<^sub>e a (\<lambda> _. F) ({t. t \<ge> 0})\<^sub>e UNIV 0 (B)\<^sub>e" (is "_ \<Longrightarrow> ?thesis1")
+  shows lie_deriv_eq: "`B \<longrightarrow> \<L>\<^bsub>F\<^esub> e on a = \<L>\<^bsub>F\<^esub> f on a` 
+  \<Longrightarrow> diff_inv_on a (\<lambda> _. F) (B)\<^sub>e ({t. t \<ge> 0})\<^sub>e UNIV 0 (e = f)\<^sub>e " (is "_ \<Longrightarrow> ?thesis1")
 proof -
-  have "`B \<longrightarrow> \<L>\<^bsub>F\<^esub> e on a = \<L>\<^bsub>F\<^esub> f on a` \<Longrightarrow> diff_inv_on (e - f = 0)\<^sub>e a (\<lambda> _. F) ({t. t \<ge> 0})\<^sub>e UNIV 0 (B)\<^sub>e"
+  have "`B \<longrightarrow> \<L>\<^bsub>F\<^esub> e on a = \<L>\<^bsub>F\<^esub> f on a` \<Longrightarrow> diff_inv_on a (\<lambda> _. F) (B)\<^sub>e ({t. t \<ge> 0})\<^sub>e UNIV 0 (e - f = 0)\<^sub>e"
     by (rule lie_diff_inv_on_eq, simp_all add: lie_deriv closure assms)
   moreover have "(e - f = 0)\<^sub>e = (e = f)\<^sub>e"
     by (simp add: expr_defs)
@@ -434,9 +435,10 @@ qed
 lemma lie_deriv_le_rule:
   fixes e :: "'s \<Rightarrow> real" and a :: "'c::real_normed_vector \<Longrightarrow> 's"
   assumes "vwb_lens a" "differentiable\<^sub>e e on a" "differentiable\<^sub>e f on a"
-  shows lie_deriv_le: "`B \<longrightarrow> \<L>\<^bsub>F\<^esub> f on a \<le> \<L>\<^bsub>F\<^esub> e on a` \<Longrightarrow> diff_inv_on (e \<ge> f)\<^sub>e a (\<lambda> _. F) ({t. t \<ge> 0})\<^sub>e UNIV 0 (B)\<^sub>e" (is "_ \<Longrightarrow> ?thesis2")
+  shows lie_deriv_le: "`B \<longrightarrow> \<L>\<^bsub>F\<^esub> f on a \<le> \<L>\<^bsub>F\<^esub> e on a` 
+  \<Longrightarrow> diff_inv_on a (\<lambda> _. F) (B)\<^sub>e ({t. t \<ge> 0})\<^sub>e UNIV 0 (e \<ge> f)\<^sub>e " (is "_ \<Longrightarrow> ?thesis2")
 proof -
-  have "`B \<longrightarrow> \<L>\<^bsub>F\<^esub> f on a \<le> \<L>\<^bsub>F\<^esub> e on a` \<Longrightarrow> diff_inv_on (e - f \<ge> 0)\<^sub>e a (\<lambda> _. F) ({t. t \<ge> 0})\<^sub>e UNIV 0 (B)\<^sub>e"
+  have "`B \<longrightarrow> \<L>\<^bsub>F\<^esub> f on a \<le> \<L>\<^bsub>F\<^esub> e on a` \<Longrightarrow> diff_inv_on a (\<lambda> _. F) (B)\<^sub>e  ({t. t \<ge> 0})\<^sub>e UNIV 0 (e - f \<ge> 0)\<^sub>e"
     by (rule lie_diff_inv_on_leq, simp_all add: lie_deriv closure assms)
   moreover have "(e - f \<ge> 0)\<^sub>e = (e \<ge> f)\<^sub>e"
     by (simp add: expr_defs)
@@ -447,9 +449,9 @@ qed
 lemma lie_deriv_less_rule:
   fixes e :: "'s \<Rightarrow> real" and a :: "'c::real_normed_vector \<Longrightarrow> 's"
   assumes "vwb_lens a" "differentiable\<^sub>e e on a" "differentiable\<^sub>e f on a"
-  shows lie_deriv_less: "`B \<longrightarrow> \<L>\<^bsub>F\<^esub> f on a \<le> \<L>\<^bsub>F\<^esub> e on a` \<Longrightarrow> diff_inv_on (e > f)\<^sub>e a (\<lambda> _. F) ({t. t \<ge> 0})\<^sub>e UNIV 0 (B)\<^sub>e" (is "_ \<Longrightarrow> ?thesis2")
+  shows lie_deriv_less: "`B \<longrightarrow> \<L>\<^bsub>F\<^esub> f on a \<le> \<L>\<^bsub>F\<^esub> e on a` \<Longrightarrow> diff_inv_on a (\<lambda> _. F) (B)\<^sub>e ({t. t \<ge> 0})\<^sub>e UNIV 0 (e > f)\<^sub>e " (is "_ \<Longrightarrow> ?thesis2")
 proof -
-  have "`B \<longrightarrow> \<L>\<^bsub>F\<^esub> f on a \<le> \<L>\<^bsub>F\<^esub> e on a` \<Longrightarrow> diff_inv_on (e - f > 0)\<^sub>e a (\<lambda> _. F) ({t. t \<ge> 0})\<^sub>e UNIV 0 (B)\<^sub>e"
+  have "`B \<longrightarrow> \<L>\<^bsub>F\<^esub> f on a \<le> \<L>\<^bsub>F\<^esub> e on a` \<Longrightarrow> diff_inv_on a (\<lambda> _. F) (B)\<^sub>e ({t. t \<ge> 0})\<^sub>e UNIV 0 (e - f > 0)\<^sub>e "
     by (rule lie_diff_inv_on_less, simp_all add: lie_deriv closure assms)
   moreover have "(e - f \<ge> 0)\<^sub>e = (e \<ge> f)\<^sub>e"
     by (simp add: expr_defs)
@@ -512,7 +514,7 @@ lemma darboux:
   apply (rule diff_ghost_rule_very_simple[where k="g/2", OF _ vwbs(3) _ zGhost])
     prefer 2 using indeps apply expr_simp
     apply (subst hoare_diff_inv_on)
-  apply (rule diff_inv_on_raw_eqI; clarsimp?)
+  apply (rule diff_inv_on_raw_eqI; (clarsimp simp: tsubst2vecf_eq)?)
   using vwbs indeps
     apply (meson lens_indep_sym plus_pres_lens_indep plus_vwb_lens) 
   using vwbs indeps apply (expr_simp add: lens_indep.lens_put_irr2)
